src/util/int32.lean
@@ -1,32 +1,35 @@
 import data.zmod.basic order.basic
 
-def int32 := zmod ⟨2^32, nat.pow_pos dec_trivial _⟩
+def int32 := zmod (2^32)
 
 namespace int32
 
+local attribute [instance]
+def int32_pos : fact (0 < 2 ^ 32) := nat.pow_pos dec_trivial _
+
 instance : has_coe int32 ℤ :=
-⟨λ i, if i.1 < 2^31 then i.1 else i.1 - 2^32⟩
+⟨λ i, if i.val < 2^31 then i.val else i.val - 2^32⟩
 
 instance : comm_ring int32 := by unfold int32; apply_instance
 
 instance : decidable_eq int32 :=
-λ x y, decidable_of_iff' _ (fin.eq_iff_veq _ _)
+λ x y, decidable_of_iff _ (zmod.val_injective _).eq_iff
 
 theorem coe_inj {i j : int32} : (i : ℤ) = j ↔ i = j :=
-⟨λ h : (ite (i.1 < 2 ^ 31) i.1 (i.1 - 2 ^ 32) : ℤ) =
-       ite (j.1 < 2 ^ 31) j.1 (j.1 - 2 ^ 32), begin
+⟨λ h : (ite (i.val < 2 ^ 31) i.val (i.val - 2 ^ 32) : ℤ) =
+       ite (j.val < 2 ^ 31) j.val (j.val - 2 ^ 32), begin
   rw ← (_ : ((2 ^ 32 : ℕ) : ℤ) = 2 ^ 32) at h,
   swap, {apply int.coe_nat_pow},
   split_ifs at h with h₁ h₂,
-  { exact fin.eq_of_veq (int.coe_nat_inj h) },
-  { have := int.coe_nat_nonneg i.1,
+  { exact zmod.val_injective _ (int.coe_nat_inj h) },
+  { have := int.coe_nat_nonneg i.val,
     rw [h, sub_nonneg, int.coe_nat_le] at this,
-    cases not_lt_of_le this j.2 },
-  { have := int.coe_nat_nonneg j.1,
+    cases not_lt_of_le this j.val_lt },
+  { have := int.coe_nat_nonneg j.val,
     rw [← h, sub_nonneg, int.coe_nat_le] at this,
-    cases not_lt_of_le this i.2 },
-  { rw sub_right_inj at h,
-    exact fin.eq_of_veq (int.coe_nat_inj h) }
+    cases not_lt_of_le this i.val_lt },
+  { rw sub_left_inj at h,
+    exact zmod.val_injective _ (int.coe_nat_inj h) }
 end, congr_arg _⟩
 
 instance : decidable_linear_order int32 :=
